arm/proofs/arm.ml
@@ -553,7 +553,12 @@ let ARM_SUBROUTINE_SIM_TAC (machinecode,execth,offset,submachinecode,subth) =
        NORMALIZE_RELATIVE_ADDRESS_CONV))] THEN
     ARM_BIGSTEP_TAC execth sname' THENL
      [MATCH_MP_TAC subimpth THEN FIRST_X_ASSUM ACCEPT_TAC;
-      ALL_TAC];;
+      ALL_TAC] THEN
+    RULE_ASSUM_TAC(CONV_RULE(TRY_CONV
+     (GEN_REWRITE_CONV I [MESON[ADD_ASSOC]
+      `read PC s = word((pc + m) + n) <=>
+       read PC s = word(pc + m + n)`] THENC
+     funpow 3 RAND_CONV NUM_ADD_CONV)));;
 
 let ARM_SUBROUTINE_SIM_ABBREV_TAC tupper ilist0 =
   let tac = ARM_SUBROUTINE_SIM_TAC tupper ilist0 in
